Partially refactor trait linking assumptions

rr_frontend/radium/src/code.rs
@@ -831,7 +831,7 @@ impl<'def> Function<'def> {
         writeln!(f, "Definition {}_lemma (π : thread_id) : Prop :=", self.name())?;
 
         // write coq parameters
-        let params = self.spec.get_all_coq_params();
+        let params = self.spec.get_all_lemma_coq_params();
         let has_params =
             !params.0.is_empty() || !self.other_functions.is_empty() || !self.used_statics.is_empty();
         if has_params {
@@ -914,13 +914,15 @@ impl<'def> Function<'def> {
         write_list!(f, &self.code.stack_layout.locals, "; ", |Variable((_, st))| st.to_string())?;
         write!(f, "] (<tag_type> ")?;
 
+        // write the specification term
         let mut scope_str = String::new();
         self.spec.generics.format(&mut scope_str, false, false, &[], &[], &[]).unwrap();
 
-        write!(f, "{scope_str} {} ", self.spec.get_spec_name())?;
+        write!(f, "{scope_str} fn_spec_add_late_pre ({} ", self.spec.get_spec_name())?;
 
         // write type args (passed to the type definition)
-        for param in &params.0 {
+        let spec_params = self.spec.get_all_spec_coq_params();
+        for param in &spec_params.0 {
             if !param.is_implicit() {
                 write!(f, "{} ", param.get_name())?;
             }
@@ -934,6 +936,30 @@ impl<'def> Function<'def> {
             write!(f, " <LFT> {}", lft)?;
         }
         write!(f, " <INST!>")?;
+
+        let late_pre = {
+            if let Some(trait_req_incl_name) = &self.spec.trait_req_incl_name {
+                let args = self.spec.get_all_trait_req_coq_params().make_using_terms();
+                let term = coq::term::App::new(trait_req_incl_name.to_owned(), args);
+
+                let mut term = term.to_string();
+                // instantiate semantic args
+                for ty in self.spec.generics.get_all_ty_params_with_assocs().params {
+                    write!(term, " <TY> {}", ty.type_term).unwrap();
+                }
+                for lft in self.spec.generics.get_lfts() {
+                    write!(term, " <LFT> {}", lft).unwrap();
+                }
+                write!(term, " <INST!>").unwrap();
+
+                term
+            } else {
+                // TODO: in this case, incl to default spec
+                "True".to_owned()
+            }
+        };
+
+        write!(f, ") (λ π, ⌜{late_pre}⌝)")?;
 
         write!(f, ").\n")
     }
@@ -952,7 +978,7 @@ impl<'def> Function<'def> {
         write!(f, "set (FN_NAME := FUNCTION_NAME \"{}\");\n", self.name())?;
 
         // intros spec params
-        let params = self.spec.get_all_coq_params();
+        let params = self.spec.get_all_lemma_coq_params();
         if !params.0.is_empty() {
             write!(f, "intros")?;
             for param in &params.0 {
@@ -1099,7 +1125,8 @@ impl<'def> Function<'def> {
                 .collect(),
         );
 
-        write!(f, "init_tyvars ({} ).\n", formatted_tyvars.as_str())
+        write!(f, "init_tyvars ({} );\n", formatted_tyvars.as_str())?;
+        write!(f, "unfold_generic_inst; simpl.\n")
     }
 
     pub fn generate_proof<F>(&self, f: &mut F, admit_proofs: bool) -> Result<(), io::Error>
@@ -1170,14 +1197,15 @@ pub struct ConstPlaceMeta<'def> {
 #[derive(Clone, Debug)]
 pub enum UsedProcedureSpec<'def> {
     /// A direct specification term.
-    Literal(String),
+    Literal(String, String),
     /// A method of a trait impl we quantify over.
     TraitMethod(QuantifiedTraitImpl<'def>, String),
 }
+
 impl<'def> Display for UsedProcedureSpec<'def> {
     fn fmt(&self, f: &mut fmt::Formatter<'_>) -> fmt::Result {
         match self {
-            Self::Literal(lit) => {
+            Self::Literal(lit, _) => {
                 write!(f, "{lit} (RRGS:=RRGS)")
             },
             Self::TraitMethod(spec_use, method_name) => {
@@ -1221,6 +1249,108 @@ pub struct UsedProcedure<'def> {
     pub syntype_of_all_args: Vec<SynType>,
 }
 
+impl<'def> UsedProcedure<'def> {
+    fn get_trait_req_incl_term(&self) -> Result<String, fmt::Error> {
+        let mut term = String::new();
+        match &self.spec_term {
+            UsedProcedureSpec::Literal(_, trait_req_incl_name) => {
+                let all_tys = self.scope_inst.get_all_ty_params_with_assocs();
+                write!(term, "{trait_req_incl_name} ")?;
+
+                // instantiate with rts and sts etc.
+                let mut gen_rfn_type_inst = Vec::new();
+                for p in &all_tys {
+                    gen_rfn_type_inst.push(format!("({})", p.get_rfn_type()));
+                }
+                // instantiate syntypes
+                for p in &all_tys {
+                    let st = SynType::from(p);
+                    gen_rfn_type_inst.push(format!("({})", st));
+                }
+                write!(term, "{} ", gen_rfn_type_inst.join(" "))?;
+
+                for x in self
+                    .scope_inst
+                    .get_surrounding_trait_requirements()
+                    .iter()
+                    .chain(self.scope_inst.get_direct_trait_requirements())
+                {
+                    write!(term, "{} ", x.get_attr_term())?;
+                    write!(term, "{} ", x.get_spec_term())?;
+                }
+
+                // instantiate lifetimes
+                for lft in self.scope_inst.get_lfts() {
+                    write!(term, " <LFT> {lft}")?;
+                }
+
+                // instantiate type variables
+                for ty in &all_tys {
+                    write!(term, " <TY> {ty}")?;
+                }
+
+                write!(term, " <INST!>")?;
+            },
+            UsedProcedureSpec::TraitMethod(trait_spec, method_name) => {
+                /*
+                let trait_ref = trait_spec.trait_ref.borrow();
+                let trait_ref = trait_ref.as_ref().unwrap();
+
+                let incl_name = &trait_ref.trait_ref.method_trait_incl_decls[method_name];
+
+                let direct_tys = self.scope_inst.get_direct_ty_params_with_assocs();
+                let trait_tys = trait_ref.get_ordered_params_inst();
+                let trait_inst = &trait_ref.trait_inst;
+
+                // how do I instantiate the requirements of the trait?
+                // - I guess I need an inst of that function's scope: scope_inst
+
+                write!(term, "{incl_name} ")?;
+
+                // TODO first instantiate with the trait's args.
+                // then with the functions' args.
+                // use trait_tys.
+
+                let mut gen_rfn_type_inst = Vec::new();
+                for p in trait_tys.iter().chain(direct_tys.iter()) {
+                    gen_rfn_type_inst.push(format!("({})", p.get_rfn_type()));
+                }
+                // instantiate syntypes
+                for p in trait_tys.iter().chain(direct_tys.iter()) {
+                    let st = SynType::from(p);
+                    gen_rfn_type_inst.push(format!("({})", st));
+                }
+                write!(term, "{} ", gen_rfn_type_inst.join(" "))?;
+
+                for x in trait_inst
+                    .get_direct_trait_requirements()
+                    .iter()
+                    .chain(self.scope_inst.get_direct_trait_requirements())
+                {
+                    write!(term, "{} ", x.get_attr_term())?;
+                    write!(term, "{} ", x.get_spec_term())?;
+                }
+
+                // instantiate lifetimes
+                for lft in trait_inst.get_lfts().iter().chain(self.scope_inst.get_lfts().iter()) {
+                    write!(term, " <LFT> {lft}")?;
+                }
+
+                // instantiate type variables
+                for ty in trait_tys.iter().chain(direct_tys.iter()) {
+                    write!(term, " <TY> {ty}")?;
+                }
+
+                write!(term, " <INST!>")?;
+                */
+
+                write!(term, "True")?;
+            },
+        }
+        Ok(term)
+    }
+}
+
 impl<'def> Display for UsedProcedure<'def> {
     fn fmt(&self, f: &mut fmt::Formatter<'_>) -> fmt::Result {
         // quantify
@@ -1230,7 +1360,6 @@ impl<'def> Display for UsedProcedure<'def> {
         let mut gen_rfn_type_inst = Vec::new();
         let all_tys = self.scope_inst.get_all_ty_params_with_assocs();
         for p in &all_tys {
-            // use an empty env, these should be closed in the current environment
             let rfn = p.get_rfn_type();
             gen_rfn_type_inst.push(format!("({})", rfn));
         }
@@ -1240,7 +1369,93 @@ impl<'def> Display for UsedProcedure<'def> {
             gen_rfn_type_inst.push(format!("({})", st));
         }
 
-        write!(f, "{} {} {} ", self.spec_term, gen_rfn_type_inst.join(" "), self.extra_spec_args.join(" "))?;
+        write!(
+            f,
+            "fn_spec_add_late_pre ({} {} {} ",
+            self.spec_term,
+            gen_rfn_type_inst.join(" "),
+            self.extra_spec_args.join(" ")
+        )?;
+
+        // TODO: add the trait incls this can assume.
+        // well, but I don't even know which trait spec this assumes....
+        // (problem: closure stuff where I need a specific pre and post!!)
+        // How does this work then?
+        // think more about that... Maybe I need to keep track of that in the frontend?
+        // I guess in the end it's a linking thing, so yeah, it makes sense that this isn't in the
+        // spec term. Also what we assume in general about other functions is a thing the frontend
+        // needs to take care of.
+        // I think this really means we should have automatic adequacy instantiation.
+        //
+        // Why do I not just put the specialized spec here directly? Then the adequacy proof
+        // becomes more difficult, because I need to subsume - that will make automation hard.
+        //
+        // I guess for every function, I should have the list of specs it assumes.
+        //
+        // Having that error put up at link time only also seems annoying.
+        //  If I assume something about a closure, then call that function, and I can't satisfy
+        //  that requirement about the closure, I want to be told at that point, not when I'm
+        //  eventually linking the whole program.
+        // => I should verify a function always against the specs its verification assumes, in order
+        //    to get reasonable errors. The verification I do should always ensure that linking
+        //    succeeds.
+        //
+        // We currently do this for functions. But for trait requirements that functions have, we
+        // need to do the same.
+        //
+        // Why is this the case?
+        // Well, I link against some specification of a trait function (I'll later instantiate this with the
+        // canonical specification, I guess) I might assume/need a different specification.
+        // So in the verification of a function, I assume that the canonical specification (that is
+        // actually verified for that function) implies the specification I need.
+        // Now, where do I dispatch that requirement?
+        //   - when I link against a function with trait requirements, I need to make sure that I instantiate
+        //     it with the right trait spec that I've actually proved. And then I need to add the obligation
+        //     that this satisfies the trait spec that the proof for that function assumes.
+        //   - what happens when I call a function of a trait that I'm generic about? I don't actually know
+        //     what the proof of the impl I link against eventually assumes. Maybe impls need to always be
+        //     generic about their trait assumptions. Otherwise, I cannot ensure that everything always links
+        //     well? Yeah, that makes sense => Otherwise, it might not imply the default spec for the trait.
+        //     Maybe the default spec for a trait should encode that. i.e. some part of our encoding should
+        //     semantically make sure of that, I think. TODO; which part enforces that?
+        //
+        //       I guess before we did that. But then we have the cylicity issues.
+        //       There seems to be a tradeoff here. We need to move these safeguards more to the
+        //       linking theorem in order to allow all this cyclicity.
+        //
+        //    For every function I use, I need to determine its trait requirements (I'm already doing that).
+        //    For each of these requirements, i need to know what specification it assumes for that.
+        //    I can export the spec term of that
+        //    However, then I need to agree on a common set of generics this depends on. It cannot
+        //    be "generics of the trait", that is too general and will rule out some specializations.
+        //    I could do "generics of the function".
+        //    Then I need to introduce a definition with the inclusions.
+        //
+        //    How does this help to break the cycle then? What is the difference to inlining it in
+        //    the specification?
+        //    - I guess in default specs this isn't included.
+        //
+        //
+        //    Problematic case: impls of two traits having a requirement for the other trait.
+        //    Then the impl's spec would be parametric in the spec of the other traits.
+        //    If I actually want to call a function and use these impls to dispatch the
+        //    requirements, I will run around a cycle.
+        //    Now: I guess the impl spec isn't parametric in the spec of the other trait anymore.
+        //      I shift the cycle into the step-indexed mutual recursion.
+        //
+        //    Specs in general are not parametric in the spec record anymore, which seems like a win.
+        //
+        //    I guess by separating it out like this, I break the cycle: the spec records are not
+        //    parametric in other spec records anymore.
+        //
+        // For trait impls that I assume, I do not have such a record. Instead, I will
+        // say that it needs the default specs.
+        // This will match the verification site as I won't allow overrides on those.
+        // TODO Q: Can I do something more specific? I could parameterize over
+        // that condition... maybe I'm kicking the can down the road then and will run
+        // into the same problem again.
+        //
+        //
 
         // apply to trait specs
         for x in self
@@ -1250,7 +1465,7 @@ impl<'def> Display for UsedProcedure<'def> {
             .chain(self.scope_inst.get_direct_trait_requirements())
         {
             write!(f, "{} ", x.get_attr_term())?;
-            write!(f, "{} ", x.get_spec_term())?;
+            //write!(f, "{} ", x.get_spec_term())?;
         }
 
         // instantiate lifetimes
@@ -1263,7 +1478,10 @@ impl<'def> Display for UsedProcedure<'def> {
             write!(f, " <TY> {ty}")?;
         }
 
-        write!(f, " <INST!>)")
+        write!(f, " <INST!>)")?;
+
+        let trait_req_term = self.get_trait_req_incl_term()?;
+        write!(f, " (λ π, ⌜{trait_req_term}⌝)%I)")
     }
 }
 
@@ -1302,9 +1520,14 @@ pub struct FunctionBuilder<'def> {
 
 impl<'def> FunctionBuilder<'def> {
     #[must_use]
-    pub fn new(name: &str, spec_name: &str) -> Self {
+    pub fn new(name: &str, spec_name: &str, trait_req_incl_name: Option<&str>) -> Self {
         let code_builder = FunctionCodeBuilder::new();
-        let spec = FunctionSpec::empty(spec_name.to_owned(), name.to_owned(), None);
+        let spec = FunctionSpec::empty(
+            spec_name.to_owned(),
+            trait_req_incl_name.map(ToOwned::to_owned),
+            name.to_owned(),
+            None,
+        );
         FunctionBuilder {
             other_functions: Vec::new(),
             code: code_builder,
