rr_frontend/translation/src/body/translation/calls.rs
@@ -127,7 +127,10 @@ impl<'a, 'def: 'a, 'tcx: 'def> TX<'a, 'def, 'tcx> {
                 .lookup_function(callee_did)
                 .ok_or_else(|| TranslationError::UnknownProcedure(format!("{:?}", callee_did)))?;
             // explicit instantiation is needed sometimes
-            let spec_term = radium::UsedProcedureSpec::Literal(meta.get_spec_name().to_owned());
+            let spec_term = radium::UsedProcedureSpec::Literal(
+                meta.get_spec_name().to_owned(),
+                meta.get_trait_req_incl_name().to_owned(),
+            );
 
             let code_name = meta.get_name();
             let loc_name = format!("{}_loc", types::mangle_name_with_tys(code_name, tup.1.as_slice()));
